cube.thy
@@ -1,0 +1,210 @@
+theory cube imports newparaGste1
+begin
+
+abbreviation c::"varType" where
+"c \<equiv>  (Ident ''c'')"
+
+abbreviation n::"varType" where
+"n \<equiv>  (Ident ''n'')"
+
+abbreviation k::"varType" where
+"k \<equiv>  (Ident ''k'')"
+
+abbreviation m::"varType" where
+"m \<equiv>  (Ident ''m'')"
+
+
+
+definition leRule::"nat \<Rightarrow> rule" where [simp]:
+"leRule N\<equiv>
+let g = uip ''<'' [IVar n, Const (index N)]  in
+let s = parallel [(c, uif ''+'' [IVar c,IVar k]),
+                  (k, uif ''+'' [IVar k,IVar m]),
+                  (m, uif ''+'' [IVar m,Const (index 6)]),
+                  (n, uif ''+'' [IVar n,Const (index 1)])]  in
+guard g s"
+
+
+consts J::" interpretFunType"  
+  
+axiomatization where axiomOnIAdd [simp,intro]:
+"  J  ''+'' [index a,   index b] = index (a + b)"
+
+axiomatization where axiomOnIMultiply [simp,intro]:
+"  J  ''*'' [index a,   index b] = index (a * b)"
+
+axiomatization where axiomOnLe [simp,intro]:  
+"  J   ''leq'' [index a, index b]  = boolV (a \<le> b)" 
+
+axiomatization where axiomOnLess [simp,intro]:  
+"  J   ''<'' [index a, index b]  = boolV (a < b)" 
+
+axiomatization where onVarn [simp,intro]:  
+"  \<exists> a. s n= (index a)"
+
+
+axiomatization where onVarc [simp,intro]:  
+"  \<exists> a. s c= (index a)"
+
+axiomatization where onVark [simp,intro]:  
+"  \<exists> a. s k= (index a)"
+
+axiomatization where onVarm [simp,intro]:  
+"  \<exists> a. s m= (index a)"
+
+subsection{*Definitions of initial states*}
+definition initSpec0::" formula" where [simp]:
+"initSpec0  \<equiv> 
+andForm (eqn (IVar m) (Const (index 6)))
+(andForm (eqn (IVar k) (Const (index 1)))
+(andForm (eqn (IVar c) (Const (index 0)))
+(eqn (IVar n) (Const (index 0)))))"
+
+definition inv1::"formula" where [simp]:
+"inv1 \<equiv>eqn ( IVar c) (uif ''*'' [(uif ''*'' [IVar n, IVar n]), IVar n])"
+
+definition inv2::"formula" where [simp]:
+"inv2\<equiv> eqn ( IVar k)
+      (uif ''+'' 
+      [(uif ''+'' [(uif ''*'' [(uif ''*'' [IVar n, IVar n]), Const (index 3)]),
+                   (uif ''*'' [IVar n,  Const (index 3)])]),
+      Const (index 1)])"
+
+definition inv3::"formula" where [simp]:
+"inv3 \<equiv> eqn (IVar m) (uif ''+'' [(uif ''*'' [IVar n,Const (index 6)]),Const (index 6)])"
+
+definition inv4::"nat \<Rightarrow> formula" where [simp]:
+"inv4 N \<equiv> uip ''leq'' [IVar n, Const (index N)]"
+
+definition invariants::"nat \<Rightarrow>formula set" where [simp]:
+"invariants N \<equiv> {inv1, inv2, inv3,inv4 N}"
+
+lemma lemmaOnInv4:
+
+shows "invHoldForRule' J s (inv4 N) (leRule N) (invariants N)"  (is "?P1 s \<or> ?P2 s \<or> ?P3 s")
+proof -
+
+  have "\<exists> a. s n=(index a)"  by simp
+    then obtain a where a1:"s n= index a" by blast
+  from a1 have "?P1 s"
+    by auto
+  then show ?thesis by auto
+qed
+    
+    
+lemma lemmaOnInv3:
+
+shows "invHoldForRule' J s (inv3 ) (leRule N) (invariants N)"   (is "?P1 s \<or> ?P2 s \<or> ?P3 s")
+proof -
+
+  have "\<exists> a. s n=(index a)"  by simp
+  then obtain a where a1:"s n= index a" by blast
+
+  have "\<exists> a. s m=(index a)"  by simp
+  then obtain a' where a2:"s m= index a'" by blast
+
+  from a1 a2 have "?P2 s"
+    by auto
+
+  then  show ?thesis  by auto
+    
+qed    
+
+lemma lemmaOnInv2:
+
+shows "invHoldForRule' J s (inv2 ) (leRule N) (invariants N)"   (is "?P1 s \<or> ?P2 s \<or> ?P3 s")
+proof -
+
+  have "\<exists> a. s n=(index a)"  by simp
+  then obtain a where a1:"s n= index a" by blast
+
+  have "\<exists> a. s k=(index a)"  by simp
+  then obtain a' where a2:"s k= index a'" by blast
+
+  from a1 a2   have "?P3 s  "
+  proof(unfold invHoldForRule4_def,rule_tac x="{inv2,inv3}" in exI,auto )qed
+
+  then show ?thesis by blast
+    
+qed    
+
+lemma lemmaOnInv1:
+
+shows "invHoldForRule' J s (inv1 ) (leRule N) (invariants N)"   (is "?P1 s \<or> ?P2 s \<or> ?P3 s")
+proof -
+
+  have "\<exists> a. s n=(index a)"  by simp
+  then obtain a where a1:"s n= index a" by blast
+
+  have "\<exists> a. s c=(index a)"  by simp
+  then obtain a' where a2:"s c= index a'" by blast
+
+  have "\<exists> a. s k=(index a)"  by simp
+  then obtain a0 where a3:"s k= index a0" by blast
+
+  have a4:"2 *(a*a) + a*a*a=(a+(a+a*a))*a"
+    by (simp add: comm_semiring_class.distrib) 
+
+  from a1 a2 a3 a4  have "?P3 s"  
+  proof(unfold invHoldForRule4_def,rule_tac x="{inv1,inv2}" in exI,simp)qed
+    
+  then   show ?thesis  by blast
+qed
+    
+
+lemma invs_on_rules:
+  assumes a1: "f \<in> invariants N" and a2: "r \<in> {leRule N} "
+  shows "invHoldForRule'  J s f r (invariants N)"
+proof -
+
+  have b1: "r=leRule N"
+    apply (cut_tac a2, auto) done
+  have "f=inv1 | f=inv2 |f=inv3 |f =inv4 N"
+    using a1 by auto 
+    moreover {
+      assume c1: "f=inv1"
+      have "invHoldForRule'  J s f r (invariants N )"
+        using b1 c1 lemmaOnInv1 by blast
+    }
+
+  moreover {
+      assume c1: "f=inv2"
+      have "invHoldForRule'  J s f r (invariants N)"
+        using b1 c1 lemmaOnInv2 by blast
+    }
+  moreover {
+      assume c1: "f=inv3"
+      have "invHoldForRule'  J s f r (invariants N)"
+        using b1 c1 lemmaOnInv3 by blast
+    }
+
+  moreover {
+      assume c1: "f=inv4 N"
+      have "invHoldForRule'  J s f r (invariants N)"
+        using b1 c1 lemmaOnInv4 by blast
+    }
+    ultimately show ?thesis by blast
+qed 
+
+lemma iniImply_inv:
+assumes a1:"f \<in> invariants N" and a2: "formEval J (initSpec0) s"
+shows "formEval J f s "
+using a1 a2 by auto
+
+lemma consistentCube: 
+  shows " consistent'  J (invariants N) {initSpec0} {leRule N}"
+proof(unfold  consistent'_def,rule conjI)
+  show "\<forall>inv ini s. inv \<in> invariants N \<longrightarrow> ini \<in> {initSpec0} \<longrightarrow> formEval J ini s \<longrightarrow> formEval J inv s"
+    using iniImply_inv by blast
+next
+  show "\<forall>inv r s. inv \<in> invariants N \<longrightarrow> r \<in> {leRule N} \<longrightarrow> invHoldForRule' J s inv r (invariants N)"
+    
+  by (smt consistent'_def iniImply_inv invs_on_rules singletonD)
+qed
+
+lemma cubeInv:
+  assumes  a2:"s \<in> reachableSet J {initSpec0}  {leRule N}" 
+  shows "\<forall> inv. inv \<in> invariants N\<longrightarrow>formEval J inv s"  (is "?P s")
+  using assms consistentCube consistentLemma' by blast
+  
+end
